concurrency/juicy/semax_preservation.v
@@ -259,7 +259,7 @@ Abort.*)
 Lemma mem_cohere_step c c' jm jm' Phi (X : rmap) ge :
   mem_cohere' (m_dry jm) Phi ->
   sepalg.join (m_phi jm) X Phi ->
-  corestep (juicy_core_sem (cl_core_sem ge)) c jm c' jm' ->
+  corestep (juicy_core_sem (Clight_core.cl_core_sem ge)) c jm c' jm' ->
   exists Phi',
     sepalg.join (m_phi jm') (age_to (level (m_phi jm')) X) Phi' /\
     mem_cohere' (m_dry jm') Phi'.
@@ -1244,7 +1244,7 @@ Admitted. (* Lemma preservation_Kinit *)
 
         (* get the next step of this particular thread (with safety for all oracles) *)
         assert (next: exists ci' jmi',
-                   corestep (juicy_core_sem (cl_core_sem ge)) ci jmi ci' jmi'
+                   corestep (juicy_core_sem (Clight_core.cl_core_sem ge)) ci jmi ci' jmi'
                    /\ forall ora, jm_bupd ora (jsafeN Jspec' ge n ora ci') jmi').
         {
           specialize (safety i cnti).
